Modified structure of vote storage and started proof

Distributed/paper_implementation.lean
@@ -1,6 +1,12 @@
 -- Structures useful to define our data structure
 namespace Model
 
+def Set (n: Nat) (T: Type) := (Fin n) -> T
+
+def updateSet [BEq T] (f: (Fin n) -> T) (i: Fin n) (t: T): (Fin n) -> T:=
+    λ x => if i == x then t else f x
+
+
 inductive Preference where 
 | Yes : Preference
 | No : Preference
@@ -11,6 +17,7 @@ inductive Decision where
 | Commit: Decision
 deriving BEq, DecidableEq
 
+
 inductive Message (n: Nat) where
 | Vote : Preference -> (Fin n) -> Message n
 | Decide : Decision -> Message n
@@ -19,13 +26,14 @@ deriving BEq, DecidableEq
 structure Coordinator (n: Nat) where
 numParticipants : Nat := n
 decision: Option Decision
-yesVotes: List Nat
-noVotes: List Nat
+yesVotes: Array Bool
+noVotes: Array Bool
 
 structure Participant (n: Nat) where
 hostid: (Fin n)
 preference: Preference
 decision: Option Decision
+deriving BEq, DecidableEq
 
 structure Network (n : Nat) where
 network: List (Message n)
@@ -33,6 +41,6 @@ network: List (Message n)
 structure System where
 n: Nat
 coordinator: Coordinator n
-participants: (Fin n) -> Participant n
+participants: Set n (Participant n)
 network: Network n
 
